Update F* extraction

libcrux-iot/ml-kem/proofs/fstar/extraction/Libcrux_iot_ml_kem.Vector.Portable.Sampling.fst
@@ -3,19 +3,19 @@ module Libcrux_iot_ml_kem.Vector.Portable.Sampling
 open Core
 open FStar.Mul
 
-let rej_sample (a: t_Slice u8) (result: t_Slice i16) =
+let rej_sample (a: t_Slice u8) (out: t_Slice i16) =
   let sampled:usize = mk_usize 0 in
-  let result, sampled:(t_Slice i16 & usize) =
+  let out, sampled:(t_Slice i16 & usize) =
     Rust_primitives.Hax.Folds.fold_range (mk_usize 0)
       ((Core.Slice.impl__len #u8 a <: usize) /! mk_usize 3 <: usize)
       (fun temp_0_ i ->
-          let result, sampled:(t_Slice i16 & usize) = temp_0_ in
+          let out, sampled:(t_Slice i16 & usize) = temp_0_ in
           let i:usize = i in
-          ((Core.Slice.impl__len #i16 result <: usize) =. mk_usize 16 <: bool) &&
+          ((Core.Slice.impl__len #i16 out <: usize) =. mk_usize 16 <: bool) &&
           (sampled <=. (mk_usize 2 *! i <: usize) <: bool))
-      (result, sampled <: (t_Slice i16 & usize))
+      (out, sampled <: (t_Slice i16 & usize))
       (fun temp_0_ i ->
-          let result, sampled:(t_Slice i16 & usize) = temp_0_ in
+          let out, sampled:(t_Slice i16 & usize) = temp_0_ in
           let i:usize = i in
           let b1:i16 =
             cast (a.[ (i *! mk_usize 3 <: usize) +! mk_usize 0 <: usize ] <: u8) <: i16
@@ -28,22 +28,22 @@ let rej_sample (a: t_Slice u8) (result: t_Slice i16) =
           in
           let d1:i16 = ((b2 &. mk_i16 15 <: i16) <<! mk_i32 8 <: i16) |. b1 in
           let d2:i16 = (b3 <<! mk_i32 4 <: i16) |. (b2 >>! mk_i32 4 <: i16) in
-          let result, sampled:(t_Slice i16 & usize) =
+          let out, sampled:(t_Slice i16 & usize) =
             if d1 <. Libcrux_iot_ml_kem.Vector.Traits.v_FIELD_MODULUS && sampled <. mk_usize 16
             then
-              let result:t_Slice i16 =
-                Rust_primitives.Hax.Monomorphized_update_at.update_at_usize result sampled d1
+              let out:t_Slice i16 =
+                Rust_primitives.Hax.Monomorphized_update_at.update_at_usize out sampled d1
               in
-              result, sampled +! mk_usize 1 <: (t_Slice i16 & usize)
-            else result, sampled <: (t_Slice i16 & usize)
+              out, sampled +! mk_usize 1 <: (t_Slice i16 & usize)
+            else out, sampled <: (t_Slice i16 & usize)
           in
           if d2 <. Libcrux_iot_ml_kem.Vector.Traits.v_FIELD_MODULUS && sampled <. mk_usize 16
           then
-            let result:t_Slice i16 =
-              Rust_primitives.Hax.Monomorphized_update_at.update_at_usize result sampled d2
+            let out:t_Slice i16 =
+              Rust_primitives.Hax.Monomorphized_update_at.update_at_usize out sampled d2
             in
-            result, sampled +! mk_usize 1 <: (t_Slice i16 & usize)
-          else result, sampled <: (t_Slice i16 & usize))
+            out, sampled +! mk_usize 1 <: (t_Slice i16 & usize)
+          else out, sampled <: (t_Slice i16 & usize))
   in
   let hax_temp_output:usize = sampled in
-  result, hax_temp_output <: (t_Slice i16 & usize)
+  out, hax_temp_output <: (t_Slice i16 & usize)
