libcrux-iot/ml-kem/proofs/fstar/extraction/Libcrux_iot_ml_kem.Vector.Portable.Sampling.fsti
@@ -3,9 +3,12 @@ module Libcrux_iot_ml_kem.Vector.Portable.Sampling
 open Core
 open FStar.Mul
 
-val rej_sample (a: t_Slice u8) (result: t_Slice i16)
+val rej_sample (a: t_Slice u8) (out: t_Slice i16)
     : Prims.Pure (t_Slice i16 & usize)
       (requires
         (Core.Slice.impl__len #u8 a <: usize) =. mk_usize 24 &&
-        (Core.Slice.impl__len #i16 result <: usize) =. mk_usize 16)
-      (fun _ -> Prims.l_True)
+        (Core.Slice.impl__len #i16 out <: usize) =. mk_usize 16)
+      (ensures
+        fun temp_0_ ->
+          let out_future, result:(t_Slice i16 & usize) = temp_0_ in
+          result <=. mk_usize 16 && (Core.Slice.impl__len #i16 out_future <: usize) =. mk_usize 16)
