libcrux-iot/ml-kem/proofs/fstar/extraction/Libcrux_iot_ml_kem.Vector.Portable.Vector_type.fst
@@ -1,0 +1,154 @@
+module Libcrux_iot_ml_kem.Vector.Portable.Vector_type
+#set-options "--fuel 0 --ifuel 1 --z3rlimit 80"
+open Core
+open FStar.Mul
+
+let _ =
+  (* This module has implicit dependencies, here we make them explicit. *)
+  (* The implicit dependencies arise from typeclasses instances. *)
+  let open Libcrux_secrets.Int in
+  let open Libcrux_secrets.Int.Public_integers in
+  let open Libcrux_secrets.Traits in
+  ()
+
+[@@ FStar.Tactics.Typeclasses.tcinstance]
+assume
+val impl_1': Core.Marker.t_Copy t_PortableVector
+
+let impl_1 = impl_1'
+
+let zero (_: Prims.unit) =
+  {
+    f_elements
+    =
+    Libcrux_secrets.Traits.f_classify #(t_Array i16 (mk_usize 16))
+      #FStar.Tactics.Typeclasses.solve
+      (Rust_primitives.Hax.repeat (mk_i16 0) (mk_usize 16) <: t_Array i16 (mk_usize 16))
+  }
+  <:
+  t_PortableVector
+
+let to_i16_array (x: t_PortableVector) (out: t_Slice i16) =
+  let _:Prims.unit =
+    if true
+    then
+      let _:Prims.unit =
+        Hax_lib.v_assert ((Core.Slice.impl__len #i16 out <: usize) >=. mk_usize 16 <: bool)
+      in
+      ()
+  in
+  let out:t_Slice i16 =
+    Rust_primitives.Hax.Monomorphized_update_at.update_at_range out
+      ({ Core.Ops.Range.f_start = mk_usize 0; Core.Ops.Range.f_end = mk_usize 16 }
+        <:
+        Core.Ops.Range.t_Range usize)
+      (Core.Slice.impl__copy_from_slice #i16
+          (out.[ { Core.Ops.Range.f_start = mk_usize 0; Core.Ops.Range.f_end = mk_usize 16 }
+              <:
+              Core.Ops.Range.t_Range usize ]
+            <:
+            t_Slice i16)
+          (Libcrux_secrets.Traits.f_declassify #(t_Array i16 (mk_usize 16))
+              #FStar.Tactics.Typeclasses.solve
+              x.f_elements
+            <:
+            t_Slice i16)
+        <:
+        t_Slice i16)
+  in
+  out
+
+let from_i16_array (array: t_Slice i16) (out: t_PortableVector) =
+  let out:t_PortableVector =
+    {
+      out with
+      f_elements
+      =
+      Core.Slice.impl__copy_from_slice #i16
+        out.f_elements
+        (array.[ { Core.Ops.Range.f_start = mk_usize 0; Core.Ops.Range.f_end = mk_usize 16 }
+            <:
+            Core.Ops.Range.t_Range usize ]
+          <:
+          t_Slice i16)
+    }
+    <:
+    t_PortableVector
+  in
+  out
+
+let from_bytes (array: t_Slice u8) (out: t_PortableVector) =
+  let out:t_PortableVector =
+    Rust_primitives.Hax.Folds.fold_range (mk_usize 0)
+      Libcrux_iot_ml_kem.Vector.Traits.v_FIELD_ELEMENTS_IN_VECTOR
+      (fun out temp_1_ ->
+          let out:t_PortableVector = out in
+          let _:usize = temp_1_ in
+          true)
+      out
+      (fun out i ->
+          let out:t_PortableVector = out in
+          let i:usize = i in
+          {
+            out with
+            f_elements
+            =
+            Rust_primitives.Hax.Monomorphized_update_at.update_at_usize out.f_elements
+              i
+              (((Libcrux_secrets.Int.f_as_i16 #u8
+                      #FStar.Tactics.Typeclasses.solve
+                      (array.[ mk_usize 2 *! i <: usize ] <: u8)
+                    <:
+                    i16) <<!
+                  mk_i32 8
+                  <:
+                  i16) |.
+                (Libcrux_secrets.Int.f_as_i16 #u8
+                    #FStar.Tactics.Typeclasses.solve
+                    (array.[ (mk_usize 2 *! i <: usize) +! mk_usize 1 <: usize ] <: u8)
+                  <:
+                  i16)
+                <:
+                i16)
+            <:
+            t_Array i16 (mk_usize 16)
+          }
+          <:
+          t_PortableVector)
+  in
+  out
+
+let to_bytes (x: t_PortableVector) (bytes: t_Slice u8) =
+  let e_bytes_len:usize = Core.Slice.impl__len #u8 bytes in
+  let bytes:t_Slice u8 =
+    Rust_primitives.Hax.Folds.fold_range (mk_usize 0)
+      Libcrux_iot_ml_kem.Vector.Traits.v_FIELD_ELEMENTS_IN_VECTOR
+      (fun bytes e_i ->
+          let bytes:t_Slice u8 = bytes in
+          let e_i:usize = e_i in
+          (Core.Slice.impl__len #u8 bytes <: usize) =. e_bytes_len <: bool)
+      bytes
+      (fun bytes i ->
+          let bytes:t_Slice u8 = bytes in
+          let i:usize = i in
+          let bytes:t_Slice u8 =
+            Rust_primitives.Hax.Monomorphized_update_at.update_at_usize bytes
+              (mk_usize 2 *! i <: usize)
+              (Libcrux_secrets.Int.f_as_u8 #i16
+                  #FStar.Tactics.Typeclasses.solve
+                  ((x.f_elements.[ i ] <: i16) >>! mk_i32 8 <: i16)
+                <:
+                u8)
+          in
+          let bytes:t_Slice u8 =
+            Rust_primitives.Hax.Monomorphized_update_at.update_at_usize bytes
+              ((mk_usize 2 *! i <: usize) +! mk_usize 1 <: usize)
+              (Libcrux_secrets.Int.f_as_u8 #i16
+                  #FStar.Tactics.Typeclasses.solve
+                  (x.f_elements.[ i ] <: i16)
+                <:
+                u8)
+          in
+          bytes)
+  in
+  bytes
